例1：
设$g(y)=\int_{2y}^{y^2}e^{-yx^2}dx,-\infty <y<+\infty$求$g'(y)$
解：因为$e^{-yx^2}$以及$de^{-yx^2}=-x^2e^{-yx^2}$在全平面上连续，$y^2与2y$在$(-\infty,+\infty)$上可导。所以$$g'(y)=-\int_{2y}^{y^2}x^2e^{-yx^2}dx+2ye^{-y^5}-2e^{-4y^3}$$

$\Gamma$函数与$B$函数
$\Gamma 函数$：$\Gamma(\alpha)=\int_0^{+\infty}x^{\alpha-1}e^{-x}dx,\alpha >0$
$\Gamma (\alpha+1)=\alpha \Gamma(\alpha)$
$\Gamma(\frac{1}{2})=\sqrt \pi$
$\Gamma(1)=1 ; \ \ \ \ \ \ \ \ \  \Gamma(n)=(n-1)!$
$B(p,q)=\int_0^{\frac{\pi}{2}}x^{2p-1}(1-x)^{2q-1}dx,\ \ \ (p>0,q>0)$
$B的常见换元：1)用x=cos^2t,2)x=\frac{t}{1+t}$
$B(p,q)=2\int_0^{\frac{\pi}{2}}sin^{2p-1}x\ cos^{2q-1}xdx=\int_0^{\infty}\frac{y^{p-1}}{{1+y}^{p+q}}dy$
$B(p,q)=B(q,p)=\frac{\Gamma(p) \cdot \Gamma(q)}{\Gamma(p+q)}$
